clib: add support for lifting global variables in `cinit`
The `cinit` and `clift` methods already provided a way to abstract
accesses to specified local variables to Isabelle variables that do not
depend on the state, provided that the procedure does not write to those
variables. The proof methods included automation of proofs that the
values of variables being abstracted remain constant throughout the
procedure.

This commit adds support for abstracting accesses to *global* variables.
The additional challenge here is that calls to other procedures might
modify global variables. We use the `modifies` facts produced by the C
parser to determine (and prove) when variables of interest are preserved
across procedure calls.

Signed-off-by: Matthew Brecknell <Matthew.Brecknell@data61.csiro.au>

proof/crefine/lib/Ctac.thy
@@ -887,40 +887,48 @@ lemma While_ceqv:
   apply simp
   done
 
-lemma call_ceqv':
-  assumes ieq: "\<And>t. rewrite_xf xf t v i i'"
-  and    ceqv: "\<And>t t' s'. ceqv \<Gamma> xf v (r t s') t' (c t s') (c' t s')" (* For record field updates *)
-  and     xf:  "\<And>t t'. xf t = v \<Longrightarrow> xf (r t t') = v"
+lemma call_ceqv_hoarep_gen:
+  assumes mod: "\<forall>s. \<Gamma>\<turnstile>\<^bsub>/F s\<^esub> (P s) Call f (Q s),(A s)"
+  assumes ieq: "\<And>s. rewrite_xf xf s v i i'"
+  and    ceqv: "\<And>t t' s'. ceqv \<Gamma> xf v (r t s') t' (c t s') (c' t s')"
+  and     xf:  "\<And>s t. xf s = v \<Longrightarrow> i' s \<in> P (x s) \<longrightarrow> t \<in> Q (x s) \<or> t \<in> A (x s) \<Longrightarrow> xf (r s t) = v"
   shows   "ceqv \<Gamma> xf v t t' (call i f r c) (call i' f r c')"
   apply (rule ceqvI)
   apply (rule iffI)
    apply (erule exec_call_Normal_elim)
-       apply (drule ceqvD1 [OF _ _ ceqv])
-        apply (simp add: xf)
+       apply (drule ceqvD1[OF _ _ ceqv])
+        apply (simp add: rewrite_xfD[OF ieq])
+        apply (erule xf)
+        apply (frule (1) hoarep_exec_call_body[OF mod], fastforce)
        apply (erule exec_call)
-        apply (simp add: rewrite_xfD [OF ieq])
+        apply (simp add: rewrite_xfD[OF ieq])
        apply assumption
-      apply (clarsimp simp: rewrite_xfD [OF ieq] elim!: exec_callAbrupt exec_callFault exec_callStuck exec_callUndefined)
-     apply (clarsimp simp: rewrite_xfD [OF ieq] elim!: exec_callAbrupt exec_callFault exec_callStuck exec_callUndefined)
-    apply (clarsimp simp: rewrite_xfD [OF ieq] elim!: exec_callAbrupt exec_callFault exec_callStuck exec_callUndefined)
-   apply (clarsimp simp: rewrite_xfD [OF ieq] elim!: exec_callAbrupt exec_callFault exec_callStuck exec_callUndefined)
-  (* clag *)
-   apply (erule exec_call_Normal_elim)
-       apply (drule ceqvD2 [OF _ _ ceqv])
-        apply (simp add: xf)
-       apply (erule exec_call)
-        apply (simp add: rewrite_xfD [OF ieq])
-       apply assumption
-      apply (clarsimp simp: rewrite_xfD [OF ieq, symmetric]
-        elim!: exec_callAbrupt exec_callFault exec_callStuck exec_callUndefined)+
+      apply (clarsimp simp: rewrite_xfD[OF ieq] elim!: exec_callAbrupt)
+     apply (clarsimp simp: rewrite_xfD[OF ieq] elim!: exec_callFault)
+    apply (clarsimp simp: rewrite_xfD[OF ieq] elim!: exec_callStuck)
+   apply (clarsimp simp: rewrite_xfD[OF ieq] elim!: exec_callUndefined)
+  apply (erule exec_call_Normal_elim)
+      apply (drule ceqvD2 [OF _ _ ceqv])
+       apply (erule xf)
+       apply (frule (1) hoarep_exec_call_body[OF mod], fastforce)
+      apply (erule exec_call)
+       apply (simp add: rewrite_xfD[OF ieq])
+      apply assumption
+     apply (clarsimp simp: rewrite_xfD[OF ieq] elim!: exec_callAbrupt)
+    apply (clarsimp simp: rewrite_xfD[OF ieq] elim!: exec_callFault)
+   apply (clarsimp simp: rewrite_xfD[OF ieq] elim!: exec_callStuck)
+  apply (clarsimp simp: rewrite_xfD[OF ieq] elim!: exec_callUndefined)
   done
 
-lemma call_ceqv:
+lemmas call_ceqv = call_ceqv_hoarep_gen[OF hoarep_false_pre_gen, simplified]
+lemmas call_ceqv_hoarep = call_ceqv_hoarep_gen[where P="\<lambda>s. {s}" and x=i and i=i for i, simplified]
+
+lemma call_ceqv':
   assumes ieq: "\<And>t. rewrite_xf xf t v i i'"
   and    ceqv: "\<And>t t' s'. ceqv \<Gamma> xf v (r t s') t' (c t s') (c' t s')" (* For record field updates *)
   and     xf:  "\<And>t t'. xf (r t t') = xf t"
   shows   "ceqv \<Gamma> xf v t t' (call i f r c) (call i' f r c')"
-  by (rule call_ceqv' [OF ieq ceqv], simp add: xf)
+  by (rule call_ceqv [OF ieq ceqv], simp add: xf)
 
 lemmas Skip_ceqv = ceqv_refl [where c = Skip]
 
@@ -1091,7 +1099,7 @@ lemmas ceqv_rules = ceqv_refl [where xf' = xfdc] \<comment> \<open>Any ceqv with
   Cond_ceqv [OF Collect_mem_eqv] Cond_UNIV_ceqv Cond_empty_ceqv
   Guard_ceqv [OF Collect_mem_eqv] Guard_UNIV_ceqv
   Seq_ceqv Seq_weak_ceqv
-  Basic_ceqv call_ceqv Skip_ceqv
+  Basic_ceqv call_ceqv' Skip_ceqv
   Catch_ceqv Throw_ceqv
   creturn_ceqv_xf creturn_ceqv_not_xf \<comment> \<open>order is important with these two, the second is more general\<close>
   ceqv_refl [where c = return_void_C] ceqv_refl [where c = break_C]
@@ -1118,10 +1126,10 @@ definition
  "ceqv_xpres_rewrite_basic xf v f f'
     \<equiv> \<forall>s. xf s = v \<longrightarrow> f s = f' s"
 
-definition
-  ceqv_xpres_basic_preserves :: "('s \<Rightarrow> 'a) \<Rightarrow> 'a \<Rightarrow> ('s \<Rightarrow> 's) \<Rightarrow> bool \<Rightarrow> bool" where
- "ceqv_xpres_basic_preserves xf v f b
-    \<equiv> b \<longrightarrow> (\<forall>s. xf s = v \<longrightarrow> xf (f s) = v)"
+definition ceqv_xpres_basic_preserves ::
+  "('s \<Rightarrow> 'v) \<Rightarrow> 'v \<Rightarrow> ('s \<Rightarrow> bool) \<Rightarrow> ('s \<Rightarrow> 's) \<Rightarrow> bool \<Rightarrow> bool"
+  where
+  "ceqv_xpres_basic_preserves xf v P f b \<equiv> b \<longrightarrow> (\<forall>s. xf s = v \<longrightarrow> P s \<longrightarrow> xf (f s) = v)"
 
 definition
   ceqv_xpres_eq_If :: "bool \<Rightarrow> 'a \<Rightarrow> 'a \<Rightarrow> 'a \<Rightarrow> bool" where
@@ -1225,7 +1233,7 @@ lemma ceqv_xpres_Seq:
 
 lemma ceqv_xpres_Basic:
   "\<lbrakk> ceqv_xpres_rewrite_basic xf v f f';
-          ceqv_xpres_basic_preserves xf v f' pres \<rbrakk>
+          ceqv_xpres_basic_preserves xf v \<top> f' pres \<rbrakk>
     \<Longrightarrow> ceqv_xpres \<Gamma> xf v True (Basic f) pres (Basic f')"
   apply (simp add: ceqv_xpres_eq_imp)
   apply (intro allI impI conjI)
@@ -1235,31 +1243,48 @@ lemma ceqv_xpres_Basic:
   apply (simp add: ceqv_xpres_basic_preserves_def)
   done
 
-lemma ceqv_xpres_call:
-  "\<lbrakk> ceqv_xpres_call_restore_args f i i';
-     ceqv_xpres_rewrite_basic xf v i' i'';
-           \<And>s'. ceqv_xpres_basic_preserves xf v (\<lambda>s. r s s') pres';
-           \<And>s' s''. ceqv_xpres \<Gamma> xf v pres' (c s' s'')  pres (c' s' s'') \<rbrakk>
-      \<Longrightarrow> ceqv_xpres \<Gamma> xf v True (call i f r c) pres (call i'' f r c')"
-  apply (simp add: ceqv_xpres_eq_imp ceqv_xpres_call_restore_args_def)
+definition ceqv_xpres_call where
+  "ceqv_xpres_call \<Gamma> xf v f r i c pres i' c'
+   \<equiv> ceqv_xpres \<Gamma> xf v True (call i f r c) pres (call i' f r c')"
+
+lemma ceqv_xpres_call_ceqv_xpres:
+  assumes "ceqv_xpres_call \<Gamma> xf v f r i c pres i' c'"
+  shows "ceqv_xpres \<Gamma> xf v True (call i f r c) pres (call i' f r c')"
+  using assms by (simp add: ceqv_xpres_call_def)
+
+lemma ceqv_xpres_call_hoarep_gen:
+  assumes mod: "\<forall>s. \<Gamma>\<turnstile>\<^bsub>/F s\<^esub> (P s) Call f (Q s),(A s)"
+  assumes args: "ceqv_xpres_call_restore_args f i i''"
+  assumes init: "ceqv_xpres_rewrite_basic xf v i'' i'"
+  assumes glob: "\<And>t. ceqv_xpres_basic_preserves xf v
+                       (\<lambda>s. i' s \<in> P (x s) \<longrightarrow> t \<in> Q (x s) \<or> t \<in> A (x s))
+                       (\<lambda>s. r s t) pres'"
+  assumes ret: "\<And>s t. ceqv_xpres \<Gamma> xf v pres' (c s t) pres (c' s t)"
+  shows "ceqv_xpres_call \<Gamma> xf v f r i c pres i' c'"
+  using init glob ret
+  apply (simp add: ceqv_xpres_call_def ceqv_xpres_eq_imp
+                   args[unfolded ceqv_xpres_call_restore_args_def, symmetric])
   apply (intro allI conjI impI)
    defer
    apply (cases pres')
-    apply (rule xpres_call)
-     apply (simp add: ceqv_xpres_basic_preserves_def)
+    apply (rule xpres_call_hoarep_gen[OF mod])
+     apply (fastforce simp: ceqv_xpres_basic_preserves_def)
     apply (simp add: ceqv_xpres_eq_imp)
    apply (simp add: ceqv_xpres_False)
   apply (cases pres')
-   apply (clarsimp simp add: ceqv_xpres_eq_imp)
-   apply (rule call_ceqv')
+   apply (clarsimp simp: ceqv_xpres_eq_imp)
+   apply (rule call_ceqv_hoarep_gen[OF mod])
      apply (simp add: rewrite_xf_def ceqv_xpres_rewrite_basic_def)
     apply simp
-   apply (simp add: ceqv_xpres_basic_preserves_def)
+   apply (fastforce simp: ceqv_xpres_rewrite_basic_def ceqv_xpres_basic_preserves_def)
   apply (simp add: ceqv_xpres_False)
-  apply (clarsimp simp add: ceqv_def ceqv_xpres_rewrite_basic_def)
-  apply (auto elim!: exec_call_Normal_elim exec_call
-                     exec_callAbrupt exec_callFault exec_callStuck exec_callUndefined)
-  done
+  apply (clarsimp simp: ceqv_def ceqv_xpres_rewrite_basic_def)
+  by (auto elim!: exec_call_Normal_elim exec_call
+                  exec_callAbrupt exec_callFault exec_callStuck exec_callUndefined)
+
+lemmas ceqv_xpres_call = ceqv_xpres_call_hoarep_gen[OF hoarep_false_pre_gen, simplified]
+lemmas ceq_xpres_call_hoarep
+  = ceqv_xpres_call_hoarep_gen[where P="\<lambda>s. {s}" and x=i' and i'=i' for i', simplified]
 
 lemma ceqv_xpres_Skip:
   "ceqv_xpres \<Gamma> xf v True Skip True Skip"
@@ -1296,9 +1321,8 @@ lemma exec_Basic_Seq_Basic:
 
 lemma ceqv_xpres_return_C:
   "\<lbrakk> ceqv_xpres_rewrite_basic xf v qf qf';
-          \<And>f. ceqv_xpres_basic_preserves xf v (xfu f) pres';
-          \<And>f. ceqv_xpres_basic_preserves xf v
-                  (global_exn_var_'_update f) pres'';
+          \<And>f. ceqv_xpres_basic_preserves xf v \<top> (xfu f) pres';
+          \<And>f. ceqv_xpres_basic_preserves xf v \<top> (global_exn_var_'_update f) pres'';
           ceqv_xpres_eq_If pres' pres'' False pres \<rbrakk>
      \<Longrightarrow> ceqv_xpres \<Gamma> xf v True (return_C xfu qf) pres (return_C xfu qf')"
   apply (simp add: ceqv_xpres_def ceqv_xpres_rewrite_basic_def
@@ -1308,11 +1332,9 @@ lemma ceqv_xpres_return_C:
   done
 
 lemma ceqv_xpres_C_bits:
-  "\<lbrakk> \<And>f. ceqv_xpres_basic_preserves xf v
-                  (global_exn_var_'_update f) pres \<rbrakk>
+  "\<lbrakk> \<And>f. ceqv_xpres_basic_preserves xf v \<top> (global_exn_var_'_update f) pres \<rbrakk>
      \<Longrightarrow> ceqv_xpres \<Gamma> xf v True return_void_C pres return_void_C"
-  "\<lbrakk> \<And>f. ceqv_xpres_basic_preserves xf v
-                  (global_exn_var_'_update f) pres \<rbrakk>
+  "\<lbrakk> \<And>f. ceqv_xpres_basic_preserves xf v \<top> (global_exn_var_'_update f) pres \<rbrakk>
      \<Longrightarrow> ceqv_xpres \<Gamma> xf v True break_C pres break_C"
   "ceqv_xpres \<Gamma> xf v True catchbrk_C True catchbrk_C"
   by (auto simp: ceqv_xpres_def
@@ -1335,7 +1357,7 @@ lemma ceqv_xpres_lvar_nondet_init:
 lemmas ceqv_xpres_rules =
   ceqv_xpres_False_pres ceqv_xpres_xfdc ceqv_xpres_whileAnno
   ceqv_xpres_While ceqv_xpres_Cond ceqv_xpres_Guard ceqv_xpres_Seq
-  ceqv_xpres_lvar_nondet_init ceqv_xpres_Basic ceqv_xpres_call
+  ceqv_xpres_lvar_nondet_init ceqv_xpres_Basic ceqv_xpres_call_ceqv_xpres
   ceqv_xpres_Skip ceqv_xpres_Catch ceqv_xpres_Throw ceqv_xpres_return_C
   ceqv_xpres_C_bits
 
@@ -1358,11 +1380,11 @@ lemma ceqv_xpres_rewrite_basic_refl:
   by (simp add: ceqv_xpres_rewrite_basic_def)
 
 lemma ceqv_xpres_basic_preserves_TrueI:
-  "\<lbrakk> \<And>s. xf s = v \<longrightarrow> xf (f s) = v \<rbrakk> \<Longrightarrow> ceqv_xpres_basic_preserves xf v f True"
+  "\<lbrakk> \<And>s. xf s = v \<longrightarrow> P s \<longrightarrow> xf (f s) = v \<rbrakk> \<Longrightarrow> ceqv_xpres_basic_preserves xf v P f True"
   by (simp add: ceqv_xpres_basic_preserves_def)
 
 lemma ceqv_xpres_basic_preserves_FalseI:
-  "ceqv_xpres_basic_preserves xf v f False"
+  "ceqv_xpres_basic_preserves xf v P f False"
   by (simp add: ceqv_xpres_basic_preserves_def)
 
 lemma ceqv_xpres_lvar_nondet_init_TrueI:
